modules/IEL/experimental/ChremaPraxis/modal/FrameSpec.v
@@ -1,3 +1,0 @@
-From Coq Require Import Program Setoids.Setoid.
-Set Implicit Arguments.
-(* ChremaPraxis FrameSpec  interface placeholder; fill with relations/flags for ChremaPraxis. *)
