modules/IEL/experimental/HexiPraxis/theorems/NormalBase.v
@@ -1,3 +1,0 @@
-From Coq Require Import Program Setoids.Setoid.
-Set Implicit Arguments.
-(* HexiPraxis NormalBase  core rules placeholder; keep constructive. *)
