modules/IEL/experimental/MuPraxis/theorems/NormalBase.v
@@ -1,8 +1,0 @@
-From Coq Require Import Program.
-(* From PXLs Require Import PXLv3.
-Require Import modules.IEL.MuPraxis.modal.FixSpec. *)
-Set Implicit Arguments.
-
-Module MuRules.
-  Definition ok := True. Lemma compiles : ok. exact I. Qed.
-End MuRules.
