modules/IEL/experimental/TychePraxis/theorems/NormalBase.v
@@ -1,8 +1,0 @@
-From Coq Require Import QArith Program.
-(* From PXLs Require Import PXLv3.
-Require Import modules.IEL.TychePraxis.modal.ProbSpec. *)
-Set Implicit Arguments.
-
-Module TycheRules.
-  Definition ok := True. Lemma compiles : ok. exact I. Qed.
-End TycheRules.
