modules/IEL/experimental/TychePraxis/theorems/Systems.v
@@ -1,2 +1,0 @@
-From Coq Require Import Program Setoids.Setoid.
-Module TychePraxisSystem. End TychePraxisSystem.
