modules/IEL/source/TheoPraxis/Core.v
@@ -1,0 +1,32 @@
+From Coq Require Import Program String Init.Datatypes.
+From PXLs Require Import PXLv3.
+From PXLs.IEL.Source.TheoPraxis Require Import Props.
+Require Import PXLs.IEL.Source.TheoPraxis.subdomains.Unity.Spec.
+Import Init.Datatypes.
+Open Scope string_scope.
+Module TheoPraxis.
+  Import TheoProps UnitySpec.
+
+  Definition V := TheoProps.Truth.
+
+  Theorem unity_foundation : forall p, V p -> p.
+  Proof. apply truth_reflect. Qed.
+
+  Theorem theological_consistency : forall p q, V p -> V q -> V (p /\ q).
+  Proof. intros p q H1 H2. unfold V in *. split; assumption. Qed.
+
+  Theorem ontological_unity : "Unity" = "Unity".
+  Proof. reflexivity. Qed.
+End TheoPraxis.
+
+(* Exported capabilities *)
+Class Cap_TheologicalFoundation : Prop := {
+  unity_foundation : forall p, TheoPraxis.V p -> p;
+  theological_consistency : forall p q, TheoPraxis.V p -> TheoPraxis.V q -> TheoPraxis.V (p /\ q);
+  ontological_unity : UnitySpec.prop_name = "Unity"
+}.
+Global Instance Cap_TheologicalFoundation_inst : Cap_TheologicalFoundation := {|
+  unity_foundation := TheoPraxis.unity_foundation;
+  theological_consistency := TheoPraxis.theological_consistency;
+  ontological_unity := TheoPraxis.ontological_unity
+|}.
